floyd/loadstore_lemmas.v
@@ -1,21 +1,13 @@
 Require Import floyd.base.
 Require Import floyd.assert_lemmas.
 Require Import floyd.client_lemmas.
+Require Import floyd.nested_field_lemmas.
+Require Import floyd.data_at_lemmas.
 Require Import floyd.field_mapsto.
 Require Import floyd.closed_lemmas.
+Require Import Coq.Logic.JMeq.
 
 Local Open Scope logic.
-
-Lemma later_left2 {T}{ND: NatDed T}{IT: Indir T}:  (* MOVE THIS TO ANOTHER FILE *)
- forall A B C : T, A && B |-- C -> A && |> B |-- |>C.
-Proof.
-intros.
-apply derives_trans with (|> (A && B)).
-rewrite later_andp.
-apply andp_derives; auto.
-apply now_later.
-apply later_derives; assumption.
-Qed.
 
 Lemma SEP_nth_isolate:
   forall n R Rn, nth_error R n = Some Rn ->
@@ -35,7 +27,6 @@ Proof.
  repeat rewrite sepcon_assoc.
  f_equal. rewrite sepcon_comm; reflexivity.
 Qed.
-
 
 Lemma SEP_replace_nth_isolate:
   forall n R Rn Rn', 
@@ -57,6 +48,143 @@ Proof.
  rewrite sepcon_assoc.
  reflexivity.
 Qed.
+
+Lemma local_andp_lemma:
+  forall P Q, P |-- local Q -> P = local Q && P.
+Proof.
+intros.
+apply pred_ext.
+apply andp_right; auto.
+apply andp_left2; auto.
+Qed.
+
+Lemma SEP_TT_right:
+  forall R, R |-- SEP(TT).
+Proof. intros. go_lowerx. rewrite sepcon_emp. apply TT_right.
+Qed.
+
+Lemma replace_nth_SEP': forall P Q R n Rn Rn' x, Rn x |-- Rn' x -> (PROPx P (LOCALx Q (SEPx (replace_nth n R Rn)))) x |-- (PROPx P (LOCALx Q (SEPx (replace_nth n R Rn')))) x.
+Proof.
+  intros.
+  normalize.
+  revert R.
+  induction n.
+  + destruct R.
+    - simpl. cancel.
+    - simpl. cancel.
+  + destruct R.
+    - simpl. cancel.
+    - intros. simpl in *. cancel.
+Qed.
+
+Lemma replace_nth_SEP: forall P Q R n Rn Rn', Rn |-- Rn' -> PROPx P (LOCALx Q (SEPx (replace_nth n R Rn))) |-- PROPx P (LOCALx Q (SEPx (replace_nth n R Rn'))).
+Proof.
+  simpl; intros.
+  apply replace_nth_SEP'.
+  apply H.
+Qed.
+
+Lemma replace_nth_SEP_andp_local': forall P Q R n Rn (Rn': environ -> mpred) Rn'' x,
+  nth_error R n = Some Rn ->
+  (PROPx P (LOCALx Q (SEPx (replace_nth n R ((`prop Rn'') && Rn'))))) x
+  = (PROPx P (LOCALx (Rn'' :: Q) (SEPx (replace_nth n R Rn')))) x.
+Proof.
+  intros.
+  normalize.
+  assert ((@fold_right (environ -> mpred) (environ -> mpred)
+              (@sepcon (environ -> mpred) (@LiftNatDed' mpred Nveric)
+                 (@LiftSepLog' mpred Nveric Sveric))
+              (@emp (environ -> mpred) (@LiftNatDed' mpred Nveric)
+                 (@LiftSepLog' mpred Nveric Sveric))
+              (@replace_nth (lifted (LiftEnviron mpred)) n R
+                 (@andp (lifted (LiftEnviron mpred))
+                    (@LiftNatDed' mpred Nveric)
+                    (@liftx (Tarrow Prop (LiftEnviron mpred))
+                       (@prop (lift_T (LiftEnviron mpred)) Nveric) Rn'') Rn'))
+              x) =
+   (@andp mpred Nveric
+           (@prop mpred Nveric
+              (Rn'' x))
+           (@fold_right (environ -> mpred) (environ -> mpred)
+              (@sepcon (environ -> mpred) (@LiftNatDed' mpred Nveric)
+                 (@LiftSepLog' mpred Nveric Sveric))
+              (@emp (environ -> mpred) (@LiftNatDed' mpred Nveric)
+                 (@LiftSepLog' mpred Nveric Sveric))
+              (@replace_nth (lifted (LiftEnviron mpred)) n R Rn') x))); 
+  [| rewrite H0; apply pred_ext; normalize].
+
+  revert R H.
+  induction n; intros.
+  + destruct R; inversion H.
+    subst l.
+    simpl. normalize.
+  + destruct R; inversion H.
+    pose proof IHn R H1.
+    unfold replace_nth in *.
+    fold (@replace_nth (LiftEnviron mpred)) in *.
+    simpl fold_right in *.
+    rewrite <- sepcon_andp_prop, H0.
+    reflexivity.
+Qed.
+
+Lemma replace_nth_SEP_andp_local: forall P Q R n Rn (Rn': environ -> mpred) Rn'',
+  nth_error R n = Some Rn ->
+  (PROPx P (LOCALx Q (SEPx (replace_nth n R ((`prop Rn'') && Rn')))))
+  = (PROPx P (LOCALx (Rn'' :: Q) (SEPx (replace_nth n R Rn')))).
+Proof.
+  intros.
+  extensionality.
+  eapply replace_nth_SEP_andp_local'.
+  exact H.
+Qed.
+
+Lemma replace_nth_nth_error: forall {A:Type} R n (Rn:A), 
+  nth_error R n = Some Rn ->
+  R = replace_nth n R Rn.
+Proof.
+  intros.
+  revert R H; induction n; intros; destruct R.
+  + reflexivity.
+  + simpl. inversion H. reflexivity.
+  + inversion H.
+  + inversion H. simpl.
+    rewrite (IHn R) at 1; simpl; [reflexivity|exact H1].
+Qed.
+
+Lemma nth_error_replace_nth: forall {A:Type} R n (Rn Rn':A), 
+  nth_error R n = Some Rn ->
+  nth_error (replace_nth n R Rn') n = Some Rn'.
+Proof.
+  intros.
+  revert R H; induction n; intros; destruct R; simpl.
+  + inversion H.
+  + inversion H.
+    reflexivity.
+  + inversion H.
+  + inversion H.
+    apply IHn, H1.
+Qed.
+
+Lemma LOCAL_2_hd: forall P Q R Q1 Q2,
+  (PROPx P (LOCALx (Q1 :: Q2 :: Q) (SEPx R))) = 
+  (PROPx P (LOCALx (Q2 :: Q1 :: Q) (SEPx R))).
+Proof.
+  intros.
+  extensionality.
+  apply pred_ext; normalize.
+Qed.
+
+(***************************************
+
+Load/store lemmas about mapsto:
+  semax_store_nth.
+  semax_store_nth'.
+  semax_load_37
+  semax_load_37'
+  semax_cast_load_37
+  semax_cast_load_37'
+
+***************************************)
 
 Lemma semax_store_nth:
 forall {Espec: OracleKind} n Delta P Q R e1 e2 Rn sh t1,
@@ -100,15 +228,879 @@ rewrite (SEP_replace_nth_isolate _ _ _ _ H0).
 auto.
 Qed.
 
-Lemma local_andp_lemma:
-  forall P Q, P |-- local Q -> P = local Q && P.
+Lemma semax_store_nth':
+  forall {Espec: OracleKind},
+    forall (n : nat) (Delta : tycontext) (P : list Prop)
+         (Q : list (environ -> Prop)) (R : list (LiftEnviron mpred))
+         (e1 e2 : expr) (Rn : LiftEnviron mpred) (sh : Share.t) 
+         (t1 : type),
+       typeof e1 = t1 ->
+       nth_error R n = Some Rn ->
+       Rn |-- `(mapsto_ sh t1) (eval_lvalue e1) ->
+       writable_share sh ->
+       PROPx P (LOCALx (tc_environ Delta :: Q) (SEPx R))
+       |-- local (tc_lvalue Delta e1) && local (tc_expr Delta (Ecast e2 t1)) ->
+       semax Delta (|>PROPx P (LOCALx Q (SEPx R))) 
+         (Sassign e1 e2)
+         (normal_ret_assert
+            (PROPx P
+               (LOCALx Q
+                  (SEPx
+                     (replace_nth n R
+                        (`(mapsto sh t1) (eval_lvalue e1)
+                           (eval_expr (Ecast e2 t1)) )))))).
 Proof.
-intros.
-apply pred_ext.
-apply andp_right; auto.
-apply andp_left2; auto.
+  intros.
+  simpl (eval_expr (Ecast e2 t1)).
+  unfold force_val1.
+  eapply semax_store_nth.
+  + exact H.
+  + exact H0.
+  + exact H1.
+  + exact H2.
+  + exact H3.
 Qed.
 
+Definition semax_load_37 := @semax_load. 
+
+Lemma semax_load_37' : 
+  forall {Espec: OracleKind},
+forall (Delta: tycontext) sh id P Q R e1 t2 (v2: val),
+    typeof_temp Delta id = Some t2 ->
+    is_neutral_cast (typeof e1) t2 = true ->
+      PROPx P (LOCALx (tc_environ Delta :: Q) (SEPx R)) |-- 
+         local (tc_lvalue Delta e1) &&
+         local (`(tc_val (typeof e1) v2)) &&
+         (`(mapsto sh (typeof e1)) (eval_lvalue e1) `v2 * TT) ->
+    @semax Espec Delta (|> PROPx P (LOCALx Q (SEPx R)))
+       (Sset id e1)
+       (normal_ret_assert (EX old:val, 
+             PROPx P 
+   (LOCALx (`eq (eval_id id) `v2 :: map (subst id (`old)) Q)
+     (SEPx (map (subst id (`old)) R))))).
+Proof.
+intros.
+eapply semax_pre_post; [ | | apply semax_load with sh t2; auto].
+* instantiate (1:= PROPx P (LOCALx Q (SEPx R))).
+  apply later_left2.
+  rewrite insert_local.
+  rewrite <- (andp_dup (PROPx P (LOCALx (_ :: _) _))).
+  eapply derives_trans.
+  apply andp_derives; [apply derives_refl | apply H1].
+  clear H.
+  go_lowerx.
+  autorewrite with gather_prop.
+  apply derives_extract_prop; intros [? ?].
+  apply andp_right.
+  apply prop_right; repeat split; try eassumption.
+  instantiate (1:= `v2). apply H5.
+  apply andp_left1; auto.
+* intros. apply andp_left2; auto.
+  apply normal_ret_assert_derives'.
+  apply exp_derives; intro old.
+  autorewrite with subst.
+  rewrite insert_local.
+  apply andp_derives; auto.
+* rewrite insert_local.
+  eapply derives_trans; [apply H1 | clear H1].
+  apply andp_left2. auto.
+Qed.
+
+Definition semax_cast_load_37 := @semax_cast_load. 
+
+Lemma semax_cast_load_37' : 
+  forall {Espec: OracleKind},
+forall (Delta: tycontext) sh id P Q R e1 t1 (v2: val),
+    typeof_temp Delta id = Some t1 ->
+      PROPx P (LOCALx (tc_environ Delta :: Q) (SEPx R)) |-- 
+         local (tc_lvalue Delta e1) &&
+         local (`(tc_val t1 (eval_cast (typeof e1) t1 v2))) &&
+         (`(mapsto sh (typeof e1)) (eval_lvalue e1) `v2 * TT) ->
+    @semax Espec Delta (|> PROPx P (LOCALx Q (SEPx R)))
+       (Sset id (Ecast e1 t1))
+       (normal_ret_assert (EX old:val, 
+             PROPx P 
+   (LOCALx (`eq (eval_id id) `(eval_cast (typeof e1) t1 v2) :: map (subst id (`old)) Q)
+     (SEPx (map (subst id (`old)) R))))).
+Proof.
+intros. rename H0 into H1; pose proof I.
+eapply semax_pre_post; [ | | apply semax_cast_load with (sh0:=sh)(v3:= `v2); auto].
+* instantiate (1:= PROPx P (LOCALx Q (SEPx R))).
+  apply later_left2.
+  rewrite insert_local.
+  rewrite <- (andp_dup (PROPx P (LOCALx (_ :: _) _))).
+  eapply derives_trans.
+  apply andp_derives; [apply derives_refl | apply H1].
+  clear H1.
+  go_lowerx.
+  autorewrite with gather_prop.
+  apply derives_extract_prop; intros [? ?].
+  apply andp_right.
+  apply prop_right; repeat split; eassumption.
+  apply andp_left1; auto.
+* intros. apply andp_left2; auto.
+  apply normal_ret_assert_derives'.
+  apply exp_derives; intro old.
+  autorewrite with subst.
+  rewrite insert_local.
+  apply andp_derives; auto.
+* rewrite insert_local.
+  eapply derives_trans; [apply H1 | clear H1].
+  apply andp_left2. auto.
+Qed.
+
+(***************************************
+
+Load/store lemmas about data_at:
+  semax_data_load.
+  semax_data_store_nth.
+
+***************************************)
+
+Lemma is_neutral_cast_by_value: forall t t', 
+  is_neutral_cast t t' = true ->
+  type_is_by_value t.
+Proof.
+  intros.
+  destruct t, t'; try inversion H; simpl; auto.
+Qed.
+
+Lemma is_neutral_reptype: forall t t', is_neutral_cast t t' = true -> reptype t = val.
+Proof.
+  intros.
+  eapply by_value_reptype, is_neutral_cast_by_value, H.
+Qed.
+
+Lemma look_up_empty_ti: forall i, look_up_ident_default i empty_ti = Tvoid.
+Proof.
+  intros.
+  unfold look_up_ident_default.
+  rewrite PTree.gempty.
+  reflexivity.
+Qed.
+
+Lemma is_neutral_data_at: forall sh t t' v v' p,
+  is_neutral_cast t t' = true ->
+  JMeq v v' ->
+  data_at sh t v p = (!! size_compatible t p) && (!! align_compatible t p) && mapsto sh t p v'.
+Proof.
+  intros.
+  apply by_value_data_at; try assumption.
+  eapply is_neutral_cast_by_value, H.
+Qed.
+
+Lemma is_neutral_lifted_data_at: forall sh t t' v (v':val) (p: environ -> val),
+  is_neutral_cast t t' = true ->
+  JMeq v v' ->
+  `(data_at sh t v) p = `prop (`(size_compatible t) p) && `prop (`(align_compatible t) p) && `(mapsto sh t) p `(v').
+Proof.
+  intros.
+  unfold liftx, lift. simpl.
+  extensionality.
+  erewrite is_neutral_data_at; [| exact H| exact H0].
+  reflexivity.
+Qed.
+
+Lemma is_neutral_data_at_: forall sh t t' p, 
+  is_neutral_cast t t' = true ->
+  data_at_ sh t p = (!! size_compatible t p) && (!! align_compatible t p) && mapsto_ sh t p.
+Proof.
+  intros.
+  apply by_value_data_at_; try assumption.
+  eapply is_neutral_cast_by_value, H.
+Qed.
+
+Lemma is_neutral_lifted_data_at_: forall sh t t' p,
+  is_neutral_cast t t' = true ->
+  `(data_at_ sh t) p = `prop (`(size_compatible t) p) &&
+  `prop (`(align_compatible t) p) && `(mapsto_ sh t) p.
+Proof.
+  intros.
+  unfold liftx, lift. simpl.
+  extensionality.
+  eapply is_neutral_data_at_; try assumption.
+  exact H.
+Qed.
+
+Lemma semax_data_load: 
+  forall {Espec: OracleKind},
+    forall (Delta : tycontext) (sh : Share.t) (id : ident) 
+         (P : list Prop) (Q : list (environ -> Prop))
+         (R : list (environ -> mpred)) (e1 : expr) 
+         (t2 : type) (v2 : reptype (typeof e1)) (v2' : val),
+       typeof_temp Delta id = Some t2 ->
+       is_neutral_cast (typeof e1) t2 = true ->
+       JMeq v2 v2' ->
+       PROPx P (LOCALx (tc_environ Delta :: Q) (SEPx R))
+       |-- local (tc_lvalue Delta e1) && local `(tc_val (typeof e1) v2') &&
+           (`(data_at sh (typeof e1) v2) (eval_lvalue e1) * TT) ->
+       semax Delta (|>PROPx P (LOCALx Q (SEPx R))) 
+         (Sset id e1)
+         (normal_ret_assert
+            (EX  old : val,
+             PROPx P
+               (LOCALx (`eq (eval_id id) `v2' :: map (subst id `old) Q)
+                  (SEPx (map (subst id `old) R))))).
+Proof.
+  intros.
+  rename H0 into Htype.
+  eapply semax_load_37'.
+  + exact H.
+  + exact Htype.
+  + instantiate (1:=sh).
+    apply (derives_trans _ _ _ H2).
+    apply andp_derives; [normalize |].
+    remember (eval_lvalue e1) as p.
+    go_lower.
+    erewrite is_neutral_data_at; [normalize| exact Htype | exact H1].
+Qed.
+
+Lemma semax_data_store_nth:
+  forall {Espec: OracleKind},
+    forall (n : nat) (Delta : tycontext) (P : list Prop)
+         (Q : list (environ -> Prop)) (R : list (LiftEnviron mpred))
+         (e1 e2 : expr) (Rn : LiftEnviron mpred) (sh : Share.t) 
+         (t1 : type) (v: val) (v' : reptype t1),
+       is_neutral_cast t1 t1 = true ->
+       JMeq v' v ->
+       typeof e1 = t1 ->
+       nth_error R n = Some Rn ->
+       Rn |-- `(data_at_ sh t1) (eval_lvalue e1) ->
+       writable_share sh ->
+       PROPx P (LOCALx (tc_environ Delta :: Q) (SEPx R))
+       |-- local (tc_lvalue Delta e1) && local (tc_expr Delta (Ecast e2 t1)) ->
+       PROPx P (LOCALx Q (SEPx (replace_nth n R (`(data_at_ sh t1) (eval_lvalue e1)) ))) |-- local (`(eq) (eval_expr (Ecast e2 t1)) `v) ->
+       semax Delta (|>PROPx P (LOCALx Q (SEPx R))) 
+         (Sassign e1 e2)
+         (normal_ret_assert
+            (PROPx P
+               (LOCALx Q
+                  (SEPx
+                     (replace_nth n R
+                        (`(data_at sh t1 v') (eval_lvalue e1)
+                          )))))).
+Proof.
+  intros until v'. intro Htype. intros.
+
+  erewrite is_neutral_lifted_data_at; [|exact Htype| exact H].
+  erewrite is_neutral_lifted_data_at_ in H2; [|exact Htype].
+  erewrite is_neutral_lifted_data_at_ in H5; [|exact Htype].
+
+  assert (Rn |-- `prop (`(size_compatible t1) (eval_lvalue e1)) &&
+                  `prop (`(align_compatible t1) (eval_lvalue e1)) && Rn) by (
+    apply andp_right; [|apply derives_refl];
+    eapply derives_trans; [exact H2|apply andp_left1; apply derives_refl]).           
+
+  eapply semax_pre0.
+  apply later_derives. Focus 1.
+  + instantiate (1:= PROPx P (LOCALx Q (SEPx (replace_nth n R (`prop (`(size_compatible t1) (eval_lvalue e1)) && `prop (`(align_compatible t1) (eval_lvalue e1)) && Rn))))).
+    rewrite (replace_nth_nth_error R _ _ H1) at 1.
+    apply replace_nth_SEP, H6.
+    
+  rewrite andp_assoc.
+  repeat (rewrite (replace_nth_SEP_andp_local P _ R n Rn); [|exact H1]).
+  rewrite <- replace_nth_nth_error.
+
+  rewrite andp_assoc.
+  repeat (rewrite (replace_nth_SEP_andp_local P _ R n Rn); [|exact H1]).
+
+  rewrite andp_assoc in H5.
+  repeat (rewrite (replace_nth_SEP_andp_local P _ R n Rn) in H5; [|exact H1]).
+
+  eapply semax_post0; [| eapply semax_store_nth'].
+  Focus 2. exact H0.
+  Focus 2. exact H1.
+  Focus 2. eapply derives_trans; [exact H2|]. apply andp_left2; apply derives_refl.
+  Focus 2. exact H3.
+  Focus 2. rewrite (replace_nth_nth_error R _ _ H1).
+           rewrite LOCAL_2_hd. rewrite <- (replace_nth_SEP_andp_local P _ R n Rn); [|exact H1].
+           rewrite LOCAL_2_hd. rewrite -> (replace_nth_SEP_andp_local P _ R n Rn); [|exact H1].
+           rewrite <- (replace_nth_nth_error R _ _ H1).
+           eapply derives_trans; [|exact H4].
+           go_lower; normalize.
+  Focus 2. exact H1.
+
+  apply normal_ret_assert_derives'.
+
+  eapply derives_trans.
+  + instantiate (1:= PROPx P
+     (LOCALx (`eq (eval_expr (Ecast e2 t1)) `v :: `(align_compatible t1) (eval_lvalue e1)
+         :: `(size_compatible t1) (eval_lvalue e1) :: Q) (SEPx (replace_nth n R (`(mapsto sh t1) (eval_lvalue e1) (eval_expr (Ecast e2 t1))))))).
+    assert (
+    PROPx P
+     (LOCALx (`(align_compatible t1) (eval_lvalue e1)
+         :: `(size_compatible t1) (eval_lvalue e1) ::Q)
+        (SEPx
+           (replace_nth n R
+              (`(mapsto sh t1) (eval_lvalue e1) (eval_expr (Ecast e2 t1))))))
+    |--
+    PROPx P
+     (LOCALx (`(align_compatible t1) (eval_lvalue e1)
+         :: `(size_compatible t1) (eval_lvalue e1) ::Q)
+        (SEPx
+           (replace_nth n R
+              (`(mapsto_ sh t1) (eval_lvalue e1)))))).
+      apply replace_nth_SEP. unfold liftx, lift. simpl. intros. apply mapsto_mapsto_.
+    unfold PROPx, LOCALx.
+    unfold PROPx, LOCALx in H5, H7.
+    simpl.
+    simpl in H5, H7.
+    intros.
+    repeat rewrite local_lift2_and in *.
+    simpl.
+    repeat try apply andp_right.
+    - apply andp_left1; cancel.
+    - eapply derives_trans; [exact (H7 x)| exact (H5 x)].
+    - apply andp_left2; apply andp_left1; apply andp_left1; cancel.
+    - apply andp_left2; apply andp_left1; apply andp_left2; apply andp_left1; cancel.
+    - apply andp_left2; apply andp_left1; apply andp_left2; apply andp_left2; cancel.
+    - apply andp_left2; apply andp_left2; cancel.
+  + rewrite <- insert_local.
+    unfold local, lift1.
+Opaque eval_expr.
+    simpl; intros.
+    remember PROPx as m.
+    normalize.
+    subst m.
+    unfold liftx, lift in H7; simpl in H7.
+Transparent eval_expr.
+    subst v.
+    apply replace_nth_SEP'.
+    unfold liftx, lift. cancel.
+Qed.
+
+(***************************************
+
+Load/store lemmas about data_at with uncompomize function on type:
+  semax_data_load'.
+  semax_data_store_nth'.
+
+***************************************)
+
+Lemma is_neutral_reptype': forall t t' t'',
+  uncompomize t = t' ->
+  is_neutral_cast t' t'' = true ->
+  reptype t = val.
+Proof.
+  intros.
+  destruct t, t', t''; try inversion H; try inversion H0; try reflexivity.
+Qed.
+
+Lemma is_neutral_data_at': forall sh t t' t'' v v' p,
+  uncompomize t = t' ->
+  is_neutral_cast t' t'' = true ->
+  JMeq v v' ->
+  data_at sh t v p =
+  (!! size_compatible (uncompomize t) p) &&
+  (!! align_compatible (uncompomize t) p) && mapsto sh t' p v'.
+Proof.
+  intros.
+  subst t'.
+  apply uncompomize_by_value_data_at; try assumption.
+  eapply is_neutral_cast_by_value, H0.
+Qed.
+
+Lemma is_neutral_lifted_data_at': forall sh t t' t'' v (v': val) p,
+  uncompomize t = t' ->
+  is_neutral_cast t' t'' = true ->
+  JMeq v v' ->
+  `(data_at sh t v) p = 
+  `prop (`(size_compatible (uncompomize t)) p) &&
+  `prop (`(align_compatible (uncompomize t)) p) && `(mapsto sh t') p `v'.
+Proof.
+  intros.
+  unfold liftx, lift. simpl.
+  extensionality.
+  eapply is_neutral_data_at'; try assumption.
+  exact H0.
+Qed.
+
+Lemma is_neutral_data_at_': forall sh t t' t'' p,
+  uncompomize t = t' ->
+  is_neutral_cast t' t'' = true ->
+  data_at_ sh t p =
+  (!! size_compatible (uncompomize t) p) &&
+  (!! align_compatible (uncompomize t) p) && mapsto_ sh t' p.
+Proof.
+  intros.
+  subst t'.
+  apply uncompomize_by_value_data_at_; try assumption.
+  eapply is_neutral_cast_by_value, H0.
+Qed.
+
+Lemma is_neutral_lifted_data_at_': forall sh t t' t'' p,
+  uncompomize t = t' ->
+  is_neutral_cast t' t'' = true ->
+  `(data_at_ sh t) p =
+  `prop (`(size_compatible (uncompomize t)) p) &&
+  `prop (`(align_compatible (uncompomize t)) p) && `(mapsto_ sh t') p.
+Proof.
+  intros.
+  unfold liftx, lift. simpl.
+  extensionality.
+  eapply is_neutral_data_at_'; try assumption.
+  exact H0.
+Qed.
+
+Lemma semax_data_load':
+  forall {Espec: OracleKind},
+    forall (Delta : tycontext) (sh : Share.t) (id : ident) 
+      (P : list Prop) (Q : list (environ -> Prop))
+      (R : list (environ -> mpred)) (e1 : expr) 
+      (t1 t2 : type) (v2 : reptype t1) (v2' : val),
+      uncompomize t1 = typeof e1 ->
+      is_neutral_cast (typeof e1) t2 = true ->
+      typeof_temp Delta id = Some t2 ->
+      JMeq v2 v2' ->
+      PROPx P (LOCALx (tc_environ Delta :: Q) (SEPx R))
+      |-- local (tc_lvalue Delta e1) && local `(tc_val (typeof e1) v2') &&
+          (`(data_at sh t1 v2) (eval_lvalue e1) * TT) ->
+      semax Delta (|>PROPx P (LOCALx Q (SEPx R))) 
+         (Sset id e1)
+         (normal_ret_assert
+            (EX  old : val,
+             PROPx P
+               (LOCALx (`eq (eval_id id) `v2' :: map (subst id `old) Q)
+                  (SEPx (map (subst id `old) R))))).
+Proof.
+  intros.
+  eapply semax_load_37'.
+  + exact H1.
+  + exact H0.
+  + instantiate (1:=sh).
+    apply (derives_trans _ _ _ H3).
+    apply andp_derives; [normalize |].
+    forget (eval_lvalue e1) as p.
+    go_lower.
+    erewrite is_neutral_data_at'; [normalize| | |]; try assumption.
+    exact H0.
+Qed.
+
+Lemma semax_data_store_nth':
+  forall {Espec: OracleKind},
+    forall (n : nat) (Delta : tycontext) (P : list Prop)
+         (Q : list (environ -> Prop)) (R : list (LiftEnviron mpred))
+         (e1 e2 : expr) (Rn : LiftEnviron mpred) (sh : Share.t) 
+         (t1 t2: type) (v: val) (v' : reptype t2),
+       uncompomize t2 = t1 ->
+       is_neutral_cast t1 t1 = true ->
+       JMeq v' v ->
+       typeof e1 = t1 ->
+       nth_error R n = Some Rn ->
+       Rn |-- `(data_at_ sh t2) (eval_lvalue e1) ->
+       writable_share sh ->
+       PROPx P (LOCALx (tc_environ Delta :: Q) (SEPx R))
+       |-- local (tc_lvalue Delta e1) && local (tc_expr Delta (Ecast e2 t1)) ->
+       PROPx P (LOCALx Q (SEPx (replace_nth n R (`(data_at_ sh t2) (eval_lvalue e1)) ))) |-- local (`(eq) (eval_expr (Ecast e2 t1)) `v) ->
+       semax Delta (|>PROPx P (LOCALx Q (SEPx R))) 
+         (Sassign e1 e2)
+         (normal_ret_assert
+            (PROPx P
+               (LOCALx Q
+                  (SEPx
+                     (replace_nth n R
+                        (`(data_at sh t2 v') (eval_lvalue e1)
+                          )))))).
+Proof.
+  intros.
+  erewrite is_neutral_lifted_data_at'; [| exact H | exact H0 | exact H1].
+  erewrite is_neutral_lifted_data_at_' in H4; [| exact H | exact H0].
+  erewrite is_neutral_lifted_data_at_' in H7; [| exact H | exact H0].
+
+  assert (Rn |-- `prop (`(size_compatible (uncompomize t2)) (eval_lvalue e1)) &&
+                  `prop (`(align_compatible (uncompomize t2)) (eval_lvalue e1)) && Rn) by (
+    apply andp_right; [|apply derives_refl];
+    eapply derives_trans; [exact H4|apply andp_left1; apply derives_refl]).           
+
+  eapply semax_pre0.
+  apply later_derives. Focus 1.
+  + instantiate (1:= PROPx P (LOCALx Q (SEPx (replace_nth n R (`prop (`(size_compatible (uncompomize t2)) (eval_lvalue e1)) && `prop (`(align_compatible (uncompomize t2)) (eval_lvalue e1)) && Rn))))).
+    rewrite (replace_nth_nth_error R _ _ H3) at 1.
+    apply replace_nth_SEP, H8.
+    
+  rewrite andp_assoc.
+  repeat (rewrite (replace_nth_SEP_andp_local P _ R n Rn); [|exact H3]).
+  rewrite <- replace_nth_nth_error.
+
+  rewrite andp_assoc.
+  repeat (rewrite (replace_nth_SEP_andp_local P _ R n Rn); [|exact H3]).
+
+  rewrite andp_assoc in H7.
+  repeat (rewrite (replace_nth_SEP_andp_local P _ R n Rn) in H7; [|exact H3]).
+
+  eapply semax_post0; [| eapply semax_store_nth'].
+  Focus 2. exact H2.
+  Focus 2. exact H3.
+  Focus 2. eapply derives_trans; [exact H4|]. apply andp_left2; apply derives_refl.
+  Focus 2. exact H5.
+  Focus 2. rewrite (replace_nth_nth_error R _ _ H3).
+           rewrite LOCAL_2_hd. rewrite <- (replace_nth_SEP_andp_local P _ R n Rn); [|exact H3].
+           rewrite LOCAL_2_hd. rewrite -> (replace_nth_SEP_andp_local P _ R n Rn); [|exact H3].
+           rewrite <- (replace_nth_nth_error R _ _ H3).
+           eapply derives_trans; [|exact H6].
+           go_lower; normalize.
+  Focus 2. exact H3.
+
+  apply normal_ret_assert_derives'.
+
+  eapply derives_trans.
+  + instantiate (1:= PROPx P
+     (LOCALx (`eq (eval_expr (Ecast e2 (uncompomize t2))) `v :: `(align_compatible (uncompomize t2)) (eval_lvalue e1)
+         :: `(size_compatible t1) (eval_lvalue e1) :: Q) (SEPx (replace_nth n R (`(mapsto sh t1) (eval_lvalue e1) (eval_expr (Ecast e2 t1))))))).
+    assert (
+    PROPx P
+     (LOCALx (`(align_compatible (uncompomize t2)) (eval_lvalue e1)
+         :: `(size_compatible (uncompomize t2)) (eval_lvalue e1) ::Q)
+        (SEPx
+           (replace_nth n R
+              (`(mapsto sh t1) (eval_lvalue e1) (eval_expr (Ecast e2 t1))))))
+    |--
+    PROPx P
+     (LOCALx (`(align_compatible (uncompomize t2)) (eval_lvalue e1)
+         :: `(size_compatible (uncompomize t2)) (eval_lvalue e1) ::Q)
+        (SEPx
+           (replace_nth n R
+              (`(mapsto_ sh t1) (eval_lvalue e1)))))).
+      apply replace_nth_SEP. unfold liftx, lift. simpl. intros. apply mapsto_mapsto_.
+    unfold PROPx, LOCALx.
+    unfold PROPx, LOCALx in H7, H9.
+    simpl.
+    simpl in H7, H9.
+    intros.
+    repeat rewrite local_lift2_and in *.
+    simpl.
+    subst t1; repeat try apply andp_right.
+    - apply andp_left1; cancel.
+    - eapply derives_trans; [exact (H9 x)|exact (H7 x)].
+    - apply andp_left2; apply andp_left1; apply andp_left1; cancel.
+    - apply andp_left2; apply andp_left1; apply andp_left2; apply andp_left1; cancel.
+    - apply andp_left2; apply andp_left1; apply andp_left2; apply andp_left2; cancel.
+    - apply andp_left2; apply andp_left2; cancel.
+  + rewrite <- insert_local.
+    unfold local, lift1.
+Opaque eval_expr.
+    simpl; intros.
+    remember PROPx as m.
+    normalize.
+    subst m.
+    unfold liftx, lift in H9; simpl in H9.
+Transparent eval_expr.
+    subst v.
+    subst t1; apply replace_nth_SEP'.
+    unfold liftx, lift. cancel.
+Qed.
+
+(********************************************
+
+Max length ids field_at load store
+
+********************************************)
+
+Fixpoint legal_nested_efield t (ids: list ident) (tts: list type) : bool :=
+  match ids, tts with
+  | nil, nil => eqb_type (uncompomize t) t
+  | nil, _ => false
+  | _ , nil => false
+  | cons id ids', cons t_ tts' => 
+    match nested_field_rec t ids with
+    | Some (_, ttt) => (legal_nested_efield t ids' tts' && 
+                       eqb_type (uncompomize ttt) t_)%bool
+    | None => false
+    end
+  end.
+
+Lemma legal_nested_efield_cons: forall id ids t tts e,
+  legal_nested_efield (typeof e) (id :: ids) (t :: tts) = true ->
+  legal_nested_efield (typeof e) ids tts = true.
+Proof.
+  intros.
+  simpl in H.
+  valid_nested_field_rec (typeof e) ids H.
+  destruct t0; inversion H; clear H2;
+  (solve_field_offset_type id f; [|inversion H]);
+  apply andb_true_iff in H;
+  destruct H;
+  rewrite H, H1;
+  reflexivity.
+Qed.
+
+Fixpoint nested_efield (e: expr) (ids: list ident) (tts: list type) : expr :=
+  match ids, tts with
+  | nil, _ => e
+  | _, nil => e
+  | cons id ids', cons t_ tts' => Efield (nested_efield e ids' tts') id t_
+  end.
+
+Fixpoint compute_nested_efield e : expr * list ident * list type :=
+  match e with
+  | Efield e' id t => 
+    match compute_nested_efield e' with
+    | (e'', ids, tts) => (e'', id :: ids, t :: tts)
+    end
+  | _ => (e, nil, nil)
+  end.
+
+Lemma compute_nested_efield_lemma: forall e,
+  match compute_nested_efield e with
+  | (e', ids, tts) => nested_efield e' ids tts = e
+  end.
+Proof.
+  intros.
+  induction e; try reflexivity.
+  simpl.
+  destruct (compute_nested_efield e) as ((?, ?), ?).
+  simpl.
+  rewrite IHe.
+  reflexivity.
+Qed.
+
+Lemma typeof_nested_efield: forall e ids tts,
+  legal_nested_efield (typeof e) ids tts = true ->
+  eqb_type (uncompomize (nested_field_type2 (typeof e) ids))
+  (typeof (nested_efield e ids tts)) = true .
+Proof.
+  intros.
+  revert tts H.
+  induction ids; intros; destruct tts; unfold nested_field_type2 in *; simpl in *.
+  + exact H.
+  + inversion H.
+  + inversion H.
+  + valid_nested_field_rec (typeof e) ids H.
+    destruct t0; inversion H; clear H2;
+    (solve_field_offset_type a f; [|inversion H]);
+    apply andb_true_iff in H;
+    destruct H as [H HH];
+    rewrite H, HH;
+    reflexivity.
+Qed.
+
+Lemma eval_lvalue_nested_efield: forall e ids tts rho,
+  legal_nested_efield (typeof e) ids tts = true ->
+  offset_val (Int.repr (nested_field_offset2 (typeof e) ids)) (eval_lvalue e rho) = 
+  offset_val Int.zero (eval_lvalue (nested_efield e ids tts) rho).
+Proof.
+  intros.
+  assert (offset_val (Int.repr (nested_field_offset2 (typeof e) ids + 0)) (eval_lvalue e rho) = 
+          offset_val (Int.repr 0) (eval_lvalue (nested_efield e ids tts) rho)); [|
+    replace (nested_field_offset2 (typeof e) ids + 0) with 
+      (nested_field_offset2 (typeof e) ids) in H0 by omega;
+    exact H0].
+  forget 0 as pos;
+  revert pos tts H.
+  induction ids; intros; destruct tts; unfold nested_field_offset2 in *; simpl.
+  + reflexivity.
+  + reflexivity.
+  + inversion H.
+  + unfold eval_field.
+    pose proof legal_nested_efield_cons _ _ _ _ _ H.
+    pose proof typeof_nested_efield _ _ _ H0.
+    unfold nested_field_type2 in H1.
+    valid_nested_field_rec (typeof e) ids H. 
+    apply eqb_type_true in H1.
+    destruct t0; inversion H; clear H4; simpl uncompomize in H1; rewrite <- H1.
+    - solve_field_offset_type a f; [|inversion H].
+      unfold liftx, lift; simpl.
+      apply andb_true_iff in H.
+      destruct H.
+      rewrite offset_offset_val, add_repr, Zplus_assoc_reverse.
+      apply (IHids _ _ H).
+    - solve_field_offset_type a f; [|inversion H].
+      unfold liftx, lift; simpl.
+      apply andb_true_iff in H.
+      destruct H.
+      rewrite <- field_mapsto.offset_val_force_ptr.
+      rewrite offset_offset_val, int_add_repr_0_l.
+      apply (IHids _ _ H).
+Qed.
+
+Lemma semax_field_load_max_path:
+  forall {Espec: OracleKind},
+    forall (Delta : tycontext) (sh : Share.t) (id : ident) 
+         (P : list Prop) (Q : list (environ -> Prop))
+         (R : list (environ -> mpred)) (e1 : expr) 
+         (t2 : type) (ids: list ident) (tts: list type)
+         (v2 : reptype (nested_field_type2 (typeof e1) ids)) (v2' : val),
+       uncompomize (nested_field_type2 (typeof e1) ids) = typeof (nested_efield e1 ids tts) ->
+       is_neutral_cast (typeof (nested_efield e1 ids tts)) t2 = true ->
+       legal_alignas_type (typeof e1) = true ->
+       legal_nested_efield (typeof e1) ids tts = true ->
+       typeof_temp Delta id = Some t2 ->
+       JMeq v2 v2' ->
+       PROPx P (LOCALx (tc_environ Delta :: Q) (SEPx R))
+       |-- local (tc_lvalue Delta (nested_efield e1 ids tts)) &&
+           local `(tc_val (typeof (nested_efield e1 ids tts)) v2') &&
+           (`(field_at sh (typeof e1) ids v2) (eval_lvalue e1) * TT) ->
+       semax Delta (|>PROPx P (LOCALx Q (SEPx R))) 
+         (Sset id (nested_efield e1 ids tts))
+         (normal_ret_assert
+            (EX  old : val,
+             PROPx P
+               (LOCALx (`eq (eval_id id) `v2' :: map (subst id `old) Q)
+                  (SEPx (map (subst id `old) R))))).
+Proof.
+  intros.
+  eapply semax_data_load'.
+  + exact H.
+  + exact H0.
+  + exact H3.
+  + exact H4.
+  + eapply derives_trans; [exact H5|].
+    instantiate (1:=sh).
+    apply andp_derives; [normalize |].
+    remember eval_lvalue as v.
+    go_lower.
+    subst v.
+    rewrite field_at_data_at; [|exact H1].
+    rewrite at_offset'_eq; [| rewrite <- data_at_offset_zero; reflexivity].
+    rewrite (eval_lvalue_nested_efield _ _ tts); [| exact H2].
+    rewrite <- data_at_offset_zero.
+    normalize.
+Qed.
+
+Lemma lower_andp_lifted_val:
+  forall (P Q: val->mpred) v, 
+  (`(P && Q) v) = (`P v && `Q v).
+Proof. reflexivity. Qed.
+
+Lemma field_at__data_at_: forall sh t ids p,
+  legal_alignas_type t = true ->
+  field_at_ sh t ids p = 
+  (!! (size_compatible t p)) &&  
+  (!! (align_compatible t p)) &&
+  (!! (isSome (nested_field_rec t ids))) && 
+  at_offset' (data_at_ sh (nested_field_type2 t ids)) (nested_field_offset2 t ids) p.
+Proof.
+  intros.
+  unfold field_at_, data_at_.
+  apply field_at_data_at, H.
+Qed.
+
+Lemma lifted_field_at_data_at: forall sh t ids v p,
+       legal_alignas_type t = true ->
+       `(field_at sh t ids v) p =
+       `prop (`(size_compatible t) p) && 
+       `prop (`(align_compatible t) p) && 
+       `prop (`(isSome (nested_field_rec t ids))) &&
+       `(at_offset' (data_at sh (nested_field_type2 t ids) v)
+         (nested_field_offset2 t ids)) p.
+Proof.
+  intros.
+  extensionality rho.
+  unfold liftx, lift; simpl.
+  apply field_at_data_at, H.
+Qed.
+
+Lemma lifted_field_at__data_at_: forall sh t ids p,
+       legal_alignas_type t = true ->
+       `(field_at_ sh t ids) p =
+       `prop (`(size_compatible t) p) && 
+       `prop (`(align_compatible t) p) && 
+       `prop (`(isSome (nested_field_rec t ids))) &&
+       `(at_offset' (data_at_ sh (nested_field_type2 t ids))
+         (nested_field_offset2 t ids)) p.
+Proof.
+  intros.
+  extensionality rho.
+  unfold liftx, lift; simpl.
+  apply field_at__data_at_, H.
+Qed.
+
+Lemma semax_field_store_nth_max_len:
+  forall {Espec: OracleKind},
+    forall (n : nat) (Delta : tycontext) (P : list Prop)
+         (Q : list (environ -> Prop)) (R : list (LiftEnviron mpred))
+         (e1 e2 : expr) (Rn : LiftEnviron mpred) (sh : Share.t) 
+         (t1: type) ids tts (v: val) (v' : reptype (nested_field_type2 (typeof e1) ids)),
+       uncompomize (nested_field_type2 (typeof e1) ids) = t1 ->
+       is_neutral_cast t1 t1 = true ->
+       legal_alignas_type (typeof e1) = true ->
+       legal_nested_efield (typeof e1) ids tts = true ->
+       JMeq v' v ->
+       typeof (nested_efield e1 ids tts) = t1 ->
+       nth_error R n = Some Rn ->
+       Rn |-- `(field_at_ sh (typeof e1) ids) (eval_lvalue e1) ->
+       writable_share sh ->
+       PROPx P (LOCALx (tc_environ Delta :: Q) (SEPx R))
+       |-- local (tc_lvalue Delta (nested_efield e1 ids tts)) && 
+           local (tc_expr Delta (Ecast e2 t1)) ->
+       PROPx P (LOCALx Q (SEPx (replace_nth n R (`(field_at_ sh (typeof e1) ids) (eval_lvalue e1)))))
+       |-- local (`(eq) (eval_expr (Ecast e2 t1)) `v) ->
+       semax Delta (|>PROPx P (LOCALx Q (SEPx R))) 
+         (Sassign (nested_efield e1 ids tts) e2)
+         (normal_ret_assert
+            (PROPx P
+               (LOCALx Q
+                  (SEPx
+                     (replace_nth n R
+                        (`(field_at sh (typeof e1) ids v') (eval_lvalue e1)
+                          )))))).
+Proof.
+  intros.
+  rewrite lifted_field_at_data_at in *; [|exact H1].
+  rewrite lifted_field_at__data_at_ in *; [|exact H1|exact H1|exact H1].
+  assert (Rn |-- 
+           `prop (`(size_compatible (typeof e1)) (eval_lvalue e1)) &&
+           `prop (`(align_compatible (typeof e1)) (eval_lvalue e1)) &&
+           `prop (`(isSome (nested_field_rec (typeof e1) ids))) && Rn).
+    apply andp_right; [apply (derives_trans _ _ _ H6) | apply derives_refl].
+    apply andp_left1; apply derives_refl.
+  rewrite (replace_nth_nth_error _ _ _ H5) at 1.
+  eapply semax_pre0; [apply later_derives, replace_nth_SEP, H10|].
+
+  rewrite andp_assoc.
+  rewrite andp_assoc.
+  repeat (rewrite (replace_nth_SEP_andp_local P _ R n Rn); [|exact H5]).
+  rewrite <- replace_nth_nth_error; [|exact H5].
+
+  rewrite andp_assoc.
+  rewrite andp_assoc.
+  repeat (rewrite (replace_nth_SEP_andp_local P _ R n Rn); [|exact H5]).
+
+  rewrite andp_assoc in H9.
+  rewrite andp_assoc in H9.
+  repeat (rewrite (replace_nth_SEP_andp_local P _ R n Rn) in H9; [|exact H5]).
+
+
+  eapply semax_post0; [| eapply semax_data_store_nth'].
+  Focus 2. exact H.
+  Focus 2. exact H0.
+  Focus 2. exact H3.
+  Focus 2. exact H4.
+  Focus 2. exact H5.
+  Focus 3. exact H7.
+  
+  + apply normal_ret_assert_derives'.
+    apply replace_nth_SEP.
+    unfold liftx, lift; simpl; intros.
+    rewrite at_offset'_eq; [| rewrite <- data_at_offset_zero; reflexivity].
+    erewrite eval_lvalue_nested_efield; [|exact H2].
+    rewrite <- data_at_offset_zero.
+    apply derives_refl.
+  + apply (derives_trans _ _ _ H6).
+    apply andp_left2.
+    unfold liftx, lift; simpl; intros.
+    rewrite at_offset'_eq; [| rewrite <- data_at__offset_zero; reflexivity].
+    erewrite eval_lvalue_nested_efield; [|exact H2].
+    rewrite <- data_at__offset_zero.
+    apply derives_refl.
+  + rewrite (replace_nth_nth_error R _ _ H5).
+    rewrite LOCAL_2_hd. rewrite <- (replace_nth_SEP_andp_local P _ R n Rn); [|exact H5].
+    rewrite LOCAL_2_hd. rewrite <- (replace_nth_SEP_andp_local P _ R n Rn); [|exact H5].
+    rewrite LOCAL_2_hd. rewrite <- (replace_nth_SEP_andp_local P _ R n Rn); [|exact H5].
+    eapply derives_trans; [|exact H8].
+    rewrite (replace_nth_nth_error R _ _ H5) at 2.
+    apply replace_nth_SEP.
+    repeat apply andp_left2; apply derives_refl.
+  + eapply derives_trans; [|exact H9].
+    apply replace_nth_SEP.
+    unfold liftx, lift; simpl; intros.
+    rewrite at_offset'_eq; [| rewrite <- data_at__offset_zero; reflexivity].
+    erewrite eval_lvalue_nested_efield; [|exact H2].
+    rewrite <- data_at__offset_zero.
+    apply derives_refl.
+Qed.
+
+(*
 Lemma semax_store_field: 
 forall Espec (Delta: tycontext) sh e1 fld P t2 e2 sid fields ,
     writable_share sh ->
@@ -245,11 +1237,6 @@ destruct (access_mode t2); try apply FF_left.
 destruct (type_is_volatile t2); try apply FF_left.
 Qed.
 
-Lemma SEP_TT_right:
-  forall R, R |-- SEP(TT).
-Proof. intros. go_lowerx. rewrite sepcon_emp. apply TT_right.
-Qed.
-
 Lemma semax_store_field_nth:
 forall Espec (Delta: tycontext) n sh t1 fld P Q R e1 e2 t2 R1 sid fields, 
     nth_error R n = Some R1 ->
@@ -295,101 +1282,6 @@ apply andp_left2.
 rewrite (SEP_replace_nth_isolate _ _ _ _ H).
 unfold exit_tycon.
 auto.
-Qed.
-
-
-(* move this to client_lemmas *)
-Lemma subst_ewand: forall i v (P Q: environ->mpred),
-  subst i v (ewand P Q) = ewand (subst i v P) (subst i v Q).
-Proof. reflexivity. Qed.
-Hint Rewrite subst_ewand : subst.
-
-Definition semax_load_37 := @semax_load. 
-
-Lemma semax_load_37' : 
-  forall {Espec: OracleKind},
-forall (Delta: tycontext) sh id P Q R e1 t2 (v2: val),
-    typeof_temp Delta id = Some t2 ->
-    is_neutral_cast (typeof e1) t2 = true ->
-      PROPx P (LOCALx (tc_environ Delta :: Q) (SEPx R)) |-- 
-         local (tc_lvalue Delta e1) &&
-         local (`(tc_val (typeof e1) v2)) &&
-         (`(mapsto sh (typeof e1)) (eval_lvalue e1) `v2 * TT) ->
-    @semax Espec Delta (|> PROPx P (LOCALx Q (SEPx R)))
-       (Sset id e1)
-       (normal_ret_assert (EX old:val, 
-             PROPx P 
-   (LOCALx (`eq (eval_id id) `v2 :: map (subst id (`old)) Q)
-     (SEPx (map (subst id (`old)) R))))).
-Proof.
-intros.
-eapply semax_pre_post; [ | | apply semax_load with sh t2; auto].
-* instantiate (1:= PROPx P (LOCALx Q (SEPx R))).
-  apply later_left2.
-  rewrite insert_local.
-  rewrite <- (andp_dup (PROPx P (LOCALx (_ :: _) _))).
-  eapply derives_trans.
-  apply andp_derives; [apply derives_refl | apply H1].
-  clear H.
-  go_lowerx.
-  autorewrite with gather_prop.
-  apply derives_extract_prop; intros [? ?].
-  apply andp_right.
-  apply prop_right; repeat split; try eassumption.
-  instantiate (1:= `v2). apply H5.
-  apply andp_left1; auto.
-* intros. apply andp_left2; auto.
-  apply normal_ret_assert_derives'.
-  apply exp_derives; intro old.
-  autorewrite with subst.
-  rewrite insert_local.
-  apply andp_derives; auto.
-* rewrite insert_local.
-  eapply derives_trans; [apply H1 | clear H1].
-  apply andp_left2. auto.
-Qed.
-
-Definition semax_cast_load_37 := @semax_cast_load. 
-
-Lemma semax_cast_load_37' : 
-  forall {Espec: OracleKind},
-forall (Delta: tycontext) sh id P Q R e1 t1 (v2: val),
-    typeof_temp Delta id = Some t1 ->
-      PROPx P (LOCALx (tc_environ Delta :: Q) (SEPx R)) |-- 
-         local (tc_lvalue Delta e1) &&
-         local (`(tc_val t1 (eval_cast (typeof e1) t1 v2))) &&
-         (`(mapsto sh (typeof e1)) (eval_lvalue e1) `v2 * TT) ->
-    @semax Espec Delta (|> PROPx P (LOCALx Q (SEPx R)))
-       (Sset id (Ecast e1 t1))
-       (normal_ret_assert (EX old:val, 
-             PROPx P 
-   (LOCALx (`eq (eval_id id) `(eval_cast (typeof e1) t1 v2) :: map (subst id (`old)) Q)
-     (SEPx (map (subst id (`old)) R))))).
-Proof.
-intros. rename H0 into H1; pose proof I.
-eapply semax_pre_post; [ | | apply semax_cast_load with (sh0:=sh)(v3:= `v2); auto].
-* instantiate (1:= PROPx P (LOCALx Q (SEPx R))).
-  apply later_left2.
-  rewrite insert_local.
-  rewrite <- (andp_dup (PROPx P (LOCALx (_ :: _) _))).
-  eapply derives_trans.
-  apply andp_derives; [apply derives_refl | apply H1].
-  clear H1.
-  go_lowerx.
-  autorewrite with gather_prop.
-  apply derives_extract_prop; intros [? ?].
-  apply andp_right.
-  apply prop_right; repeat split; eassumption.
-  apply andp_left1; auto.
-* intros. apply andp_left2; auto.
-  apply normal_ret_assert_derives'.
-  apply exp_derives; intro old.
-  autorewrite with subst.
-  rewrite insert_local.
-  apply andp_derives; auto.
-* rewrite insert_local.
-  eapply derives_trans; [apply H1 | clear H1].
-  apply andp_left2. auto.
 Qed.
 
 Lemma semax_load_field'':
@@ -681,4 +1573,4 @@ go_lowerx.
 unfold_lift. rewrite field_at_force_ptr.
 apply derives_refl.
 Qed.
-
+*)
