floyd/client_lemmas.v
@@ -2838,4 +2838,19 @@ Ltac drop_LOCAL n :=
    first [apply (drop_LOCAL n) | apply (drop_LOCAL' n)];
     unfold delete_nth.
 
+Lemma later_left2 {T}{ND: NatDed T}{IT: Indir T}:
+ forall A B C : T, A && B |-- C -> A && |> B |-- |>C.
+Proof.
+intros.
+apply derives_trans with (|> (A && B)).
+rewrite later_andp.
+apply andp_derives; auto.
+apply now_later.
+apply later_derives; assumption.
+Qed.
+
+Lemma subst_ewand: forall i v (P Q: environ->mpred),
+  subst i v (ewand P Q) = ewand (subst i v P) (subst i v Q).
+Proof. reflexivity. Qed.
+Hint Rewrite subst_ewand : subst.
 
